source for two labs

PnP2023/Labs/Lab02/SelectionSort.lean
@@ -1,9 +1,13 @@
 import PnP2023.Lec_01_20.NatMin
 
 /-!
-# Selection sort
+# Selection sort (part 1)
 
 Selection sort is a simple sorting algorithm. It works by repeatedly finding the minimum element and moving it to the front. In this lab, you will implement selection sort in Lean (building on the `smallest` function defined in the lectures) and prove its basic properties. 
+
+You will implement this in two labs (this one and the next). In this lab, you will implement the `selectionSort` function and prove termination. In the next lab, you will prove that the function is correct, i.e., `selectionSort` preserves membership list and the result is sorted.
+
+__Note:__ If the list has duplicates the sorted list will erase these. For example, `[1, 1, 2, 3]` will be sorted to `[1, 2, 3]`. For the purposes of this exercise, this is fine.
 -/
 
 /-!
@@ -17,7 +21,14 @@ def remove (a : α) : List α → List α
 ```
 -/
 
+-- For your convenience, here are some definitions/theorems that may be useful in the two labs. Clicking on them takes you to the source, where you may find other useful results.
 #check List.remove -- {α : Type u_1} → [inst : DecidableEq α] → α → List α → List α
+#check List.length_cons -- ∀ {α : Type u_1} (a : α) (as : List α), List.length (a :: as) = Nat.succ (List.length as)
+#check List.mem_cons -- ∀ {α : Type u_1} {a b : α} {l : List α}, a ∈ b :: l ↔ a = b ∨ a ∈ l
+#check List.mem_of_mem_remove -- ∀ {α : Type u_1} [inst : DecidableEq α] {a b : α} {as : List α}, b ∈ List.remove a as → b ∈ as
+#check List.remove_eq_of_not_mem -- ∀ {α : Type u_1} [inst : DecidableEq α] {a : α} {as : List α}, ¬a ∈ as → List.remove a as = as
+#check List.mem_remove_iff -- ∀ {α : Type u_1} [inst : DecidableEq α] {a b : α} {as : List α}, b ∈ List.remove a as ↔ b ∈ as ∧ b ≠ a
+
 
 /-! 
 We will work throughout with lists of natural numbers.
@@ -25,11 +36,17 @@ We will work throughout with lists of natural numbers.
 - Problem 1: Prove the following theorem (remove the sorry)
 -/
 
-/-- Removing an element from a list shortens the list -/
-theorem remove_mem_length {a : ℕ} {l : List ℕ} (h : a ∈ l) : (List.remove a l).length < l.length  := by sorry
+/-- Removing an element from a list does not increase length -/
+theorem remove_length_le (a : ℕ) (l : List ℕ) : (List.remove a l).length ≤ l.length := by 
+  sorry
+
+
+/-- Removing a member from a list shortens the list -/
+theorem remove_mem_length {a : ℕ} {l : List ℕ} (hyp : a ∈ l) : (List.remove a l).length < l.length  := by 
+  sorry
 
 /-!
-- Problem 2: Prove termination of the following definition (remove the sorry). You may wish to remove the `decreasing_by` line.
+- Problem 3: Prove termination of the following definition (remove the sorry). You may wish to remove the `decreasing_by` line.
 -/
 /-- The selection sort function -/
 def selectionSort (l : List ℕ) : List ℕ := 
@@ -37,30 +54,4 @@ def selectionSort (l : List ℕ) : List ℕ :=
     (smallest l c) :: selectionSort (List.remove (smallest l c) l)
 termination_by _ _ => l.length
 decreasing_by sorry
-
-/-!
-We now define recursively when a list is sorted. -/
-
-/-- A direct definition of an element being below all members of a list. -/
-def List.le_all (a : ℕ) (l : List ℕ) : Prop := ∀ b: ℕ, b ∈ l → a ≤ b
-
-/-- Whether a given list is sorted. -/
-def List.sorted: List ℕ →  Prop 
-| [] => True 
-| h :: t => (t.le_all h) ∧ (t.sorted)
-
-/-!
-- Problem 3 show that the selection sort function gives a sorted list(remove sorry). 
--/
-
-/-- Selection sort is sorted -/
-theorem selectionSort_sorted (l : List ℕ) : (selectionSort l).sorted := by sorry
-
-/-!
-- Problems 4, 5: Prove that the selection sort function preserves membership (remove both the sorries).
--/
-theorem selectionSort_mem (l : List ℕ) (a : ℕ) : a ∈ l ↔ a ∈ selectionSort l := by 
-  apply Iff.intro
-  · sorry
-  · sorry
 
