PnP2023/Labs/Lab02/AnswerLE.lean
@@ -1,0 +1,6 @@
+import PnP2023.Lec_01_25.Answer
+
+namespace Waffle
+
+theorem Answer.eq_of_le_le (a b  : Answer) : 
+  a ≤ b → b ≤ a → a = b := by  sorry
