PnP2023/Labs/Lab03/SelectionSort.lean
@@ -1,0 +1,58 @@
+import PnP2023.Labs.Lab02.SelectionSort
+
+/-!
+# Selection Sort (continued)
+
+In this lab you will show that `selectionSort` defined in the previous lab is correct, i.e. the result is sorted and preserves membership.
+
+__Note:__ If the list has duplicates the sorted list will erase these. For example, `[1, 1, 2, 3]` will be sorted to `[1, 2, 3]`. For the purposes of this exercise, this is fine.
+
+
+We first define recursively when a list is sorted. -/
+
+/-- A direct definition of an element being below all members of a list. -/
+def List.le_all (a : ℕ) (l : List ℕ) : Prop := ∀ b: ℕ, b ∈ l → a ≤ b
+
+/-- Whether a given list is sorted. -/
+def List.sorted: List ℕ →  Prop 
+| [] => True 
+| h :: t => (t.le_all h) ∧ (t.sorted)
+
+-- For your convenience, here are some definitions/theorems that may be useful in the two labs. Clicking on them takes you to the source, where you may find other useful results.
+#check List.remove -- {α : Type u_1} → [inst : DecidableEq α] → α → List α → List α
+#check List.length_cons -- ∀ {α : Type u_1} (a : α) (as : List α), List.length (a :: as) = Nat.succ (List.length as)
+#check List.mem_cons -- ∀ {α : Type u_1} {a b : α} {l : List α}, a ∈ b :: l ↔ a = b ∨ a ∈ l
+#check List.mem_of_mem_remove -- ∀ {α : Type u_1} [inst : DecidableEq α] {a b : α} {as : List α}, b ∈ List.remove a as → b ∈ as
+#check List.remove_eq_of_not_mem -- ∀ {α : Type u_1} [inst : DecidableEq α] {a : α} {as : List α}, ¬a ∈ as → List.remove a as = as
+#check List.mem_remove_iff -- ∀ {α : Type u_1} [inst : DecidableEq α] {a b : α} {as : List α}, b ∈ List.remove a as ↔ b ∈ as ∧ b ≠ a
+
+/-!
+- Problem 1: show that members of the given list are members of the sorted list(remove sorry). 
+-/
+
+/-- Members of a list are members of the given sorted list -/
+theorem selectionSort_mem_of_mem {a : ℕ} {l : List ℕ} (hyp : a ∈ l) : a ∈ selectionSort l := by 
+  sorry
+
+/-!
+- Problem 2: show that members of the sorted list are members of the given list(remove sorry). 
+-/
+
+/-- Members of the sorted list are members of the given list -/
+theorem selectionSort_mem_mem {a : ℕ} {l : List ℕ} (hyp : a ∈ selectionSort l) : a ∈ l := by 
+  sorry
+
+theorem selectionSort_mem (l : List ℕ) (a : ℕ) : a ∈ l ↔ a ∈ selectionSort l := by 
+  apply Iff.intro
+  · apply selectionSort_mem_of_mem
+  · apply selectionSort_mem_mem
+
+/-!
+- Problems 3: Prove that the results of `selectionSort` is sorted (remove the sorry).
+-/
+
+
+/-- The result of `selectionSort` is sorted -/
+theorem selectionSort_sorted (l : List ℕ) : (selectionSort l).sorted := 
+    by sorry
+      
